Drop resolve

theories/Sem/Wp.v
@@ -54,28 +54,26 @@ Definition SP (Q : val -> mpred) (v : val) (free : FreeTemps) : mpred :=
 
 (* evaluate an expression as an lvalue *)
 Parameter wp_lval
-  : forall {resolve : genv},
-    thread_info -> region ->
+  : thread_info -> region ->
     Expr ->
     (val -> FreeTemps -> epred) -> (* result -> free -> post *)
     mpred. (* pre-condition *)
 
-Axiom Proper_wp_lval : forall resolve ti r e,
+Axiom Proper_wp_lval : forall ti r e,
     Proper ((pointwise_relation _ (pointwise_relation _ lentails)) ==> lentails)
-           (@wp_lval resolve ti r e).
+           (@wp_lval ti r e).
 Global Existing Instance Proper_wp_lval.
 
 (* evaluate an expression as an prvalue *)
 Parameter wp_prval
-  : forall {resolve : genv},
-    thread_info -> region ->
+  : thread_info -> region ->
     Expr ->
     (val -> FreeTemps -> epred) -> (* result -> free -> post *)
     mpred. (* pre-condition *)
 
-Axiom Proper_wp_prval : forall resolve ti r e,
+Axiom Proper_wp_prval : forall ti r e,
     Proper ((pointwise_relation _ (pointwise_relation _ lentails)) ==> lentails)
-           (@wp_prval resolve ti r e).
+           (@wp_prval ti r e).
 Global Existing Instance Proper_wp_prval.
 
 (* evaluate an initializing expression
@@ -84,36 +82,34 @@ Global Existing Instance Proper_wp_prval.
  *    https://en.cppreference.com/w/cpp/language/value_category)
  *)
 Parameter wp_init
-  : forall {resolve : genv},
-    thread_info -> region ->
+  : thread_info -> region ->
     type -> val -> Expr ->
     (FreeTemps -> epred) -> (* free -> post *)
     mpred. (* pre-condition *)
-Axiom Proper_wp_init : forall resolve ti r ty addr e,
+Axiom Proper_wp_init : forall ti r ty addr e,
     Proper (pointwise_relation _ lentails ==> lentails)
-           (@wp_init resolve ti r ty addr e).
+           (@wp_init ti r ty addr e).
 Global Existing Instance Proper_wp_init.
 
 
 (* evaluate an expression as an xvalue *)
 Parameter wp_xval
-  : forall {resolve : genv},
-    thread_info -> region ->
+  : thread_info -> region ->
     Expr ->
     (val -> FreeTemps -> epred) -> (* result -> free -> post *)
     mpred. (* pre-condition *)
 
-Axiom Proper_wp_xval : forall resolve ti r e,
+Axiom Proper_wp_xval : forall ti r e,
     Proper ((pointwise_relation _ (pointwise_relation _ lentails)) ==> lentails)
-           (@wp_xval resolve ti r e).
+           (@wp_xval ti r e).
 Global Existing Instance Proper_wp_xval.
 
-Definition wp_glval {resolve : genv} (ti : thread_info) (r : region) e Q :=
-  wp_lval (resolve:=resolve) ti r e Q \\//
-  wp_xval (resolve:=resolve) ti r e Q.
-Theorem Proper_wp_glval : forall resolve ti r e,
+Definition wp_glval (ti : thread_info) (r : region) e Q :=
+  wp_lval ti r e Q \\//
+  wp_xval ti r e Q.
+Theorem Proper_wp_glval : forall ti r e,
     Proper ((pointwise_relation _ (pointwise_relation _ lentails)) ==> lentails)
-           (@wp_glval resolve ti r e).
+           (@wp_glval ti r e).
 Proof.
   unfold wp_glval; simpl. do 2 red. intros.
   rewrite -> H. eauto.
@@ -121,12 +117,12 @@ Qed.
 Global Existing Instance Proper_wp_glval.
 
 
-Definition wp_rval {resolve : genv} (ti : thread_info) (r : region) e Q :=
-  wp_prval (resolve:=resolve) ti r e Q \\//
-  wp_xval (resolve:=resolve) ti r e Q.
-Theorem Proper_wp_rval : forall resolve ti r e,
+Definition wp_rval (ti : thread_info) (r : region) e Q :=
+  wp_prval ti r e Q \\//
+  wp_xval ti r e Q.
+Theorem Proper_wp_rval : forall ti r e,
     Proper ((pointwise_relation _ (pointwise_relation _ lentails)) ==> lentails)
-           (@wp_rval resolve ti r e).
+           (@wp_rval ti r e).
 Proof.
   unfold wp_rval; simpl. do 2 red. intros.
   rewrite -> H. eauto.
@@ -134,16 +130,15 @@ Qed.
 Global Existing Instance Proper_wp_rval.
 
 Section wpe.
-  Context {resolve : genv}.
   Variable ti : thread_info.
   Variable ρ : region.
 
   Definition wpe (vc : ValCat)
   : Expr -> (val -> FreeTemps -> mpred) -> mpred :=
     match vc with
-    | Lvalue => @wp_lval resolve ti ρ
-    | Rvalue => @wp_prval resolve ti ρ
-    | Xvalue => @wp_xval resolve ti ρ
+    | Lvalue => @wp_lval ti ρ
+    | Rvalue => @wp_prval ti ρ
+    | Xvalue => @wp_xval ti ρ
     end.
 
   Definition wpAny (vce : ValCat * Expr)
@@ -246,11 +241,11 @@ Qed.
 
 (* evaluate a statement *)
 Parameter wp
-  : forall {resolve : genv}, thread_info -> region -> Stmt -> Kpreds -> mpred.
+  : thread_info -> region -> Stmt -> Kpreds -> mpred.
 
-Axiom Proper_wp : forall resolve ti r e,
+Axiom Proper_wp : forall ti r e,
     Proper (equiv ==> lentails)
-           (@wp resolve ti r e).
+           (wp ti r e).
 Global Existing Instance Proper_wp.
 
 (* note: the [list val] here represents the *locations* of the parameters, not
@@ -258,22 +253,23 @@ Global Existing Instance Proper_wp.
  * todo(gmm): this isn't currently true, but it should be true
  *)
 Parameter func_ok_raw
-  : forall {resolve: genv}, thread_info -> Func -> list val -> (val -> mpred) -> mpred.
+  : thread_info -> Func -> list val -> (val -> mpred) -> mpred.
 
 (* todo(gmm): this is because func_ok is implemented using wp. *)
 Axiom func_ok_raw_conseq:
-  forall {resolve} ti f vs (Q Q' : val -> mpred),
+  forall ti f vs (Q Q' : val -> mpred),
     (forall r : val, Q r |-- Q' r) ->
-    func_ok_raw (resolve:=resolve) ti f vs Q |-- func_ok_raw (resolve:=resolve) ti f vs Q'.
+    func_ok_raw ti f vs Q |-- func_ok_raw ti f vs Q'.
 
-Definition fspec {resolve} (n : val) (ls : list val) (ti : thread_info) (Q : val -> mpred) : mpred :=
+
+Definition fspec (n : val) (ls : list val) (ti : thread_info) (Q : val -> mpred) : mpred :=
   Exists f, [| n = Vptr f |] **
-  Exists func, code_at func f ** func_ok_raw (resolve:=resolve) ti func ls Q.
+  Exists func, code_at func f ** func_ok_raw ti func ls Q.
 
 Theorem fspec_ok_conseq:
-  forall {resolve} (p : val) (vs : list val) ti (K m : val -> mpred),
+  forall (p : val) (vs : list val) ti (K m : val -> mpred),
     (forall r : val, m r |-- K r) ->
-    fspec (resolve:=resolve) p vs ti m |-- fspec (resolve:=resolve) p vs ti K.
+    fspec p vs ti m |-- fspec p vs ti K.
 Proof.
   intros. unfold fspec.
   iIntros "H". iDestruct "H" as (f) "[-> H]".
