theories/Sem/Atomic.v
@@ -29,7 +29,7 @@ Section with_Σ.
   (****** Wp Semantics for atomic operations
    * These are given in the style of function call axioms
    *)
-  Parameter wp_atom : forall {resolve:genv},
+  Parameter wp_atom :
       AtomicOp -> type (* the access type of the atomic operation *) ->
       list val -> (val -> mpred) -> mpred.
 
@@ -48,14 +48,14 @@ Section with_Σ.
   (* note that this rule captures all of the interesting reasoning about atomics
    * through the use of [wp_shift]
    *)
-  Axiom wp_prval_atomic: forall rslv ti r ao es ty Q,
+  Axiom wp_prval_atomic: forall ti r ao es ty Q,
       match get_acc_type ao ty (map (fun x => type_of (snd x)) es) with
       | None => lfalse
       | Some acc_type =>
-        wp_args (resolve:=rslv) ti r es (fun (vs : list val) (free : FreeTemps) =>
-          wrap_shift (wp_atom (resolve:=rslv) ao acc_type vs) (fun v => Q v free))
+        wp_args ti r es (fun (vs : list val) (free : FreeTemps) =>
+          wrap_shift (wp_atom ao acc_type vs) (fun v => Q v free))
       end
-      |-- wp_prval (resolve:=rslv) ti r (Eatomic ao es ty) Q.
+      |-- wp_prval ti r (Eatomic ao es ty) Q.
 
   (* Memory Ordering Patterns: Now we only have _SEQ_CST *)
   Definition _SEQ_CST := Vint 5.
@@ -71,34 +71,34 @@ Section with_Σ.
    * because all of the invariant reasoning is encapsulated in [wp_shift].
    *)
   Axiom wp_atom_load_cst
-  : forall rslv q memorder (acc_type:type) (l : val) (Q : val -> mpred),
+  : forall q memorder (acc_type:type) (l : val) (Q : val -> mpred),
       [| memorder = _SEQ_CST |] **
       |> (Exists v, (_at (_eq l) (tprim acc_type q v) **
                      (_at (_eq l) (tprim acc_type q v) -* Q v)))
-      |-- wp_atom (resolve:=rslv) AO__atomic_load_n acc_type (l :: memorder :: nil) Q.
+      |-- wp_atom AO__atomic_load_n acc_type (l :: memorder :: nil) Q.
 
   Axiom wp_atom_store_cst
-  : forall rslv memorder acc_type l Q v,
+  : forall memorder acc_type l Q v,
       [| memorder = _SEQ_CST |] **
       [| has_type v acc_type |] **
       |> (_at (_eq l) (tany acc_type 1) **
          (_at (_eq l) (tprim acc_type 1 v) -* Exists void, Q void))
-      |-- wp_atom (resolve:=rslv) AO__atomic_store_n acc_type (l :: memorder :: v :: nil) Q.
+      |-- wp_atom AO__atomic_store_n acc_type (l :: memorder :: v :: nil) Q.
 
   (* atomic compare and exchange n *)
   Axiom wp_atom_compare_exchange_n_suc:
-    forall rslv val_p expected_p desired wk succmemord failmemord Q' ty v,
+    forall val_p expected_p desired wk succmemord failmemord Q' ty v,
       [| wk = Vbool false |] ** [| succmemord = _SEQ_CST |] **
       [| failmemord = _SEQ_CST |] **
       |> (_at (_eq expected_p) (tprim ty 1 v) **
           _at (_eq val_p) (tprim ty 1 v) **
           ((_at (_eq expected_p) (tprim ty 1 v) **
             _at (_eq val_p) (tprim ty 1 desired)) -* Q' (Vbool true)))
-      |-- wp_atom (resolve:=rslv) AO__atomic_compare_exchange_n ty
+      |-- wp_atom AO__atomic_compare_exchange_n ty
                   (val_p::succmemord::expected_p::failmemord::desired::wk::nil) Q'.
 
   Axiom wp_atom_compare_exchange_n_fail:
-    forall rslv val_p expected_p desired wk succmemord failmemord Q'
+    forall val_p expected_p desired wk succmemord failmemord Q'
            (ty : type) v expected,
       [|wk = Vbool false|] ** [|succmemord = _SEQ_CST|] ** [| failmemord = _SEQ_CST |] **
       [| v <> expected |] **
@@ -106,7 +106,7 @@ Section with_Σ.
           _at (_eq val_p) (tprim ty 1 v) **
           ((_at (_eq expected_p) (tprim ty 1 v) **
             _at (_eq val_p) (tprim ty 1 v)) -* Q' (Vbool false)))
-      |-- wp_atom (resolve:=rslv) AO__atomic_compare_exchange_n ty
+      |-- wp_atom AO__atomic_compare_exchange_n ty
                   (val_p::succmemord::expected_p::failmemord::desired::wk::nil) Q'.
 
 (*
@@ -129,7 +129,7 @@ Section with_Σ.
 *)
 
   Axiom wp_atom_compare_exchange_suc :
-    forall rslv q val_p expected_p desired_p wk succmemord failmemord Q
+    forall q val_p expected_p desired_p wk succmemord failmemord Q
       (ty : type)
       expected desired,
       [|wk = Vbool false|] ** [|succmemord = _SEQ_CST|] ** [| failmemord = _SEQ_CST |] **
@@ -139,11 +139,11 @@ Section with_Σ.
          ((_at (_eq expected_p) (tprim ty 1 expected) **
            _at (_eq desired_p) (tprim ty q desired) **
            _at (_eq val_p) (tprim ty 1 desired)) -* Q (Vbool true)))
-       |-- wp_atom (resolve:=rslv) AO__atomic_compare_exchange ty
+       |-- wp_atom AO__atomic_compare_exchange ty
                    (val_p::succmemord::expected_p::failmemord::desired_p::wk::nil) Q.
 
   Axiom wp_atom_compare_exchange_fail :
-    forall rslv q val_p expected_p desired_p wk succmemord failmemord Q
+    forall q val_p expected_p desired_p wk succmemord failmemord Q
       (ty : type)
       actual expected desired,
       expected <> actual ->
@@ -154,7 +154,7 @@ Section with_Σ.
           ((_at (_eq expected_p) (tprim ty 1 actual) **
             _at (_eq desired_p) (tprim ty q desired) **
             _at (_eq val_p) (tprim ty 1 actual)) -* Q (Vbool false)))
-       |-- wp_atom (resolve:=rslv) AO__atomic_compare_exchange ty
+       |-- wp_atom AO__atomic_compare_exchange ty
                    (val_p::succmemord::expected_p::failmemord::desired_p::wk::nil) Q.
 
 (*
@@ -185,14 +185,14 @@ Section with_Σ.
 
   (* atomic fetch and xxx rule *)
   Definition wp_fetch_xxx ao op : Prop :=
-    forall rslv E pls memorder Q sz sgn v,
+    forall E pls memorder Q sz sgn v,
       let acc_type := Tint sz sgn in
       ([| memorder = _SEQ_CST |] **
        |> _at (_eq E) (tprim acc_type 1 v) **
        |> (Exists v',
-         [| eval_binop (resolve:=rslv) op acc_type acc_type acc_type v pls v' |] **
+           Sem.Logic.L.eval_binop op acc_type acc_type acc_type v pls v' **
          (_at (_eq E) (tprim acc_type 1 v') -* Q v))
-      |-- wp_atom (resolve:=rslv) ao acc_type (E::memorder::pls::nil) Q).
+      |-- wp_atom ao acc_type (E::memorder::pls::nil) Q).
 
   Ltac fetch_xxx ao op :=
     let G := eval unfold wp_fetch_xxx in (wp_fetch_xxx ao op) in exact G.
@@ -205,14 +205,14 @@ Section with_Σ.
 
   (* atomic xxx and fetch rule *)
   Definition wp_xxx_fetch ao op : Prop :=
-    forall rslv E pls memorder Q sz sgn,
+    forall E pls memorder Q sz sgn,
       let acc_type := Tint sz sgn in
       ([| memorder = _SEQ_CST |] **
       |> (Exists v,
           _at (_eq E) (tprim acc_type 1 v) **
-          Exists v', [| eval_binop (resolve:=rslv) op acc_type acc_type acc_type v pls v' |] **
+          Exists v', Sem.Logic.L.eval_binop op acc_type acc_type acc_type v pls v' **
                      (_at (_eq E) (tprim acc_type 1 v') -* Q v'))
-      |-- wp_atom (resolve:=rslv) ao acc_type (E::memorder::pls::nil) Q).
+      |-- wp_atom ao acc_type (E::memorder::pls::nil) Q).
 
 (*
   Definition wp_xxx_fetch ao op : Prop :=
