theories/Sem/Call.v
@@ -19,20 +19,19 @@ Module Type Call.
 
   Section with_resolve.
     Context {Σ:gFunctors}.
-    Context {resolve : genv}.
     Variable ti : thread_info.
     Variable ρ : region.
 
-    Local Notation wp := (wp (Σ:=Σ) (resolve:=resolve)  ti ρ).
-    Local Notation wpe := (wpe (Σ:=Σ) (resolve:=resolve) ti ρ).
-    Local Notation wp_lval := (wp_lval (Σ:=Σ) (resolve:=resolve) ti ρ).
-    Local Notation wp_rval := (wp_rval (Σ:=Σ) (resolve:=resolve) ti ρ).
-    Local Notation wp_prval := (wp_prval (Σ:=Σ) (resolve:=resolve) ti ρ).
-    Local Notation wp_xval := (wp_xval (Σ:=Σ) (resolve:=resolve) ti ρ).
-    Local Notation wp_init := (wp_init (Σ:=Σ) (resolve:=resolve) ti ρ).
-    Local Notation wpAny := (wpAny (Σ:=Σ) (resolve:=resolve) ti ρ).
-    Local Notation wpAnys := (wpAnys (Σ:=Σ) (resolve:=resolve) ti ρ).
-    Local Notation fspec := (fspec (Σ:=Σ) (resolve:=resolve)).
+    Local Notation wp := (wp (Σ:=Σ) ti ρ).
+    Local Notation wpe := (wpe (Σ:=Σ) ti ρ).
+    Local Notation wp_lval := (wp_lval (Σ:=Σ) ti ρ).
+    Local Notation wp_rval := (wp_rval (Σ:=Σ) ti ρ).
+    Local Notation wp_prval := (wp_prval (Σ:=Σ) ti ρ).
+    Local Notation wp_xval := (wp_xval (Σ:=Σ) ti ρ).
+    Local Notation wp_init := (wp_init (Σ:=Σ) ti ρ).
+    Local Notation wpAny := (wpAny (Σ:=Σ) ti ρ).
+    Local Notation wpAnys := (wpAnys (Σ:=Σ) ti ρ).
+    Local Notation fspec := (fspec (Σ:=Σ)).
 
     Local Notation mpred := (mpred Σ) (only parsing).
     Local Notation FreeTemps := (FreeTemps Σ) (only parsing).
@@ -51,7 +50,7 @@ Module Type Call.
             Forall a, _at (_eq a) (uninit (erase_qualifiers ty) 1) -*
                       let (e,dt) := destructor_for e in
                       wp_init ty a e (fun free => wp_args es (fun vs frees =>
-                                                             Q (a :: vs) (mdestroy (resolve:=resolve) ti ty a dt free ** frees)))
+                                                             Q (a :: vs) (mdestroy ti ty a dt free ** frees)))
           else
             wp_prval e (fun v free => wp_args es (fun vs frees =>
                                                 Q (v :: vs) (free ** frees)))
