theories/Sem/Deinit.v
@@ -14,18 +14,17 @@ Module Type Deinit.
 
   Section with_resolve.
     Context {Σ:gFunctors}.
-    Context {resolve : genv}.
     Variable ti : thread_info.
     Variable ρ : region.
 
-    Local Notation wp := (wp (Σ:=Σ) (resolve:=resolve)  ti ρ).
-    Local Notation wpe := (wpe (Σ:=Σ) (resolve:=resolve) ti ρ).
-    Local Notation wp_lval := (wp_lval (Σ:=Σ) (resolve:=resolve) ti ρ).
-    Local Notation wp_rval := (wp_rval (Σ:=Σ) (resolve:=resolve) ti ρ).
-    Local Notation wp_xval := (wp_xval (Σ:=Σ) (resolve:=resolve) ti ρ).
-    Local Notation wpAny := (wpAny (Σ:=Σ) (resolve:=resolve) ti ρ).
-    Local Notation wpAnys := (wpAnys (Σ:=Σ) (resolve:=resolve) ti ρ).
-    Local Notation fspec := (fspec (Σ:=Σ) (resolve:=resolve)).
+    Local Notation wp := (wp (Σ:=Σ)  ti ρ).
+    Local Notation wpe := (wpe (Σ:=Σ) ti ρ).
+    Local Notation wp_lval := (wp_lval (Σ:=Σ) ti ρ).
+    Local Notation wp_rval := (wp_rval (Σ:=Σ) ti ρ).
+    Local Notation wp_xval := (wp_xval (Σ:=Σ) ti ρ).
+    Local Notation wpAny := (wpAny (Σ:=Σ) ti ρ).
+    Local Notation wpAnys := (wpAnys (Σ:=Σ) ti ρ).
+    Local Notation fspec := (fspec (Σ:=Σ)).
 
     Local Notation mpred := (mpred Σ) (only parsing).
     Local Notation Rep := (Rep Σ) (only parsing).
@@ -36,7 +35,7 @@ Module Type Deinit.
      *  destructors *in the right order*
      *)
     Parameter wpd
-      : forall {resolve : genv} (ti : thread_info) (ρ : region)
+      : forall (ti : thread_info) (ρ : region)
           (cls : globname) (this : val)
           (init : FieldOrBase * obj_name)
           (Q : mpred), mpred.
@@ -47,7 +46,7 @@ Module Type Deinit.
              (Q : mpred) : mpred :=
       match dests with
       | nil => Q
-      | d :: ds => @wpd resolve ti ρ cls this d (wpds cls this ds Q)
+      | d :: ds => @wpd ti ρ cls this d (wpds cls this ds Q)
       end.
 
     Axiom wpd_deinit : forall cls this path dn Q,
@@ -55,7 +54,7 @@ Module Type Deinit.
            (_global dn &~ dp **
             _offsetL (offset_for cls path) (_eq this) &~ fp ** ltrue) //\\
                    |> fspec dp (this :: nil) ti (fun _ => Q)
-        |-- wpd (resolve:=resolve) ti ρ cls this (path, dn) Q.
+        |-- wpd ti ρ cls this (path, dn) Q.
 
   End with_resolve.
 
